refinements/DropBranchPredictors.v
@@ -7,6 +7,33 @@ Require Import Proc.AbstractIsa Proc.Fetch Proc.Decode Proc.Execute Proc.InOrder
 Set Implicit Arguments.
 Open Scope string.
 
+(** TODO: move to the general place *)
+Require Import FunctionalExtensionality.
+
+Section DropMeths.
+  Variable dropMeths: list string.
+
+  Definition dropMeths_vp (n: string) (v: (sigT SignT)): option (sigT SignT) :=
+    if in_dec string_dec n dropMeths
+    then None
+    else Some v.
+
+  Definition dropMeths_p (cs: MethsT) := M.complement cs dropMeths.
+
+  Lemma dropMeths_vp_p:
+    liftToMap1 dropMeths_vp = dropMeths_p.
+  Proof.
+    extensionality cs.
+    M.ext x.
+    unfold dropMeths_vp, dropMeths_p.
+    rewrite SemFacts.liftToMap1_find.
+    rewrite M.complement_find.
+    change M.F.P.F.eq_dec with string_dec.
+    destruct (in_dec string_dec x dropMeths); findeq.
+  Qed.
+
+End DropMeths.
+
 Section Processor.
   Variables addrSize dataBytes rfIdx: nat.
 
@@ -14,7 +41,10 @@ Section Processor.
   Variable execInst: ExecT addrSize dataBytes rfIdx.
 
   Variables btbIndexSize btbTagSize bhtIndexSize bhtTrainSize: nat.
-  Hypothesis (Hbtb: btbIndexSize + btbTagSize = addrSize).
+  Variables (getIndex: forall {ty}, fullType ty (SyntaxKind (Bit addrSize)) ->
+                                    Expr ty (SyntaxKind (Bit btbIndexSize)))
+            (getTag: forall {ty}, fullType ty (SyntaxKind (Bit addrSize)) ->
+                                  Expr ty (SyntaxKind (Bit btbTagSize))).
 
   (** Fetch related *)
   Definition fetchNondet := fetchNondet addrSize dataBytes f2iName.
@@ -62,9 +92,7 @@ Section Processor.
      writeback)%kami.
    *)
   Definition inOrderEight :=
-    inOrderEight decodeInst execInst
-                 btbIndexSize btbTagSize bhtIndexSize bhtTrainSize
-                 Hbtb.
+    inOrderEight decodeInst execInst bhtIndexSize bhtTrainSize getIndex getTag.
 
   Definition inOrderEight0 :=
     (fetchNondet ++ decRedir ++ exeRedir ++ decEpoch ++ exeEpoch ++ f2i ++
@@ -99,17 +127,55 @@ Section Processor.
     (*                    if in_dec string_dec e ndefs then nl else e :: nl) pdefs nil) as ddefs. *)
     (* compute in ddefs. *)
 
-    Local Definition p (n: string) (v: (sigT SignT)): option (sigT SignT) :=
-      if in_dec string_dec n dropMeths
-      then None
-      else Some v.
+    Local Definition p := dropMeths_vp dropMeths.
 
     Local Definition ruleMap (o: RegsT) (n: string) : option string := Some n.
-    
+
+    Ltac equiv_label_map :=
+      repeat
+        match goal with
+        | [ |- EquivalentLabelMapElem _ _ _] =>
+          unfold EquivalentLabelMapElem;
+          let H := fresh "H" in
+          intros ? H ?; vm_compute in H
+        | [H: _ \/ _ |- _] => destruct H; subst
+        | [H: False |- _] => inversion H
+        end; try reflexivity.
+
     Theorem inOrderEight_inOrderEight0: inOrderEight <<== inOrderEight0.
     Proof.
-      (* apply traceRefines_labelMap_weakening with (vp:= p); [kequiv| |]. *)
-      (* apply decompositionDrop with (theta:= theta) (ruleMap:= ruleMap). *)
+      apply traceRefines_labelMap_weakening with (vp:= p);
+        [kequiv| |equiv_label_map].
+
+      apply decompositionDrop with (theta:= theta) (ruleMap:= ruleMap).
+      - kequiv.
+      - vm_compute; tauto.
+      - vm_compute; tauto.
+      - intros.
+        unfold p.
+        pose proof (dropMeths_vp_p dropMeths); rewrite H0.
+        apply M.complement_Disj; auto.
+      - meqReify.
+      - meqReify.
+      - intros; apply M.complement_union.
+      - intros; apply M.complement_Disj; auto.
+      - (** TODO: just need one trivial invariant: a state always has register 
+         * values initially defined. *)
+        admit.
+
+        (* With the above invariant, below should work. *)
+        (* intros. *)
+        (* kinvert. *)
+        (* + kinv_action_dest; *)
+        (*     kinv_custom idtac; *)
+        (*     kinv_regmap_red; *)
+        (*     kinv_constr; *)
+        (*     kinv_eq. *)
+      - (** TODO: just need one trivial invariant: a state always has register 
+         * values initially defined. *)
+
+        (* Confirmed kinv_magic works fast enough for drop cases *)
+        admit.
     Admitted.
 
   End Refinement.
